Picinae_mstatics.v
@@ -1,0 +1,805 @@
+(* Picinae: Platform In Coq for INstruction Analysis of Executables       ZZM7DZ
+                                                                          $MNDM7
+   Copyright (c) 2026 Kevin W. Hamlen            ,,A??=P                 OMMNMZ+
+   The University of Texas at Dallas         =:$ZZ$+ZZI                  7MMZMZ7
+   Computer Science Department             Z$$ZM++O++                    7MMZZN+
+                                          ZZ$7Z.ZM~?                     7MZDNO$
+                                        ?Z8ZO7.OM=+?                     $OMO+Z+
+   Any use, commercial or otherwise       ?D=++M++ZMMNDNDZZ$$Z?           MM,IZ=
+   requires the express permission of        MZZZZZZ+...=.8NOZ8NZ$7       MM+$7M
+   the author.                                 ?NNMMM+.IZDMMMMZMD8O77     O7+MZ+
+                                                     MMM8MMMMMMMMMMM77   +MMMMZZ
+                                                     MMMMMMMMMMMZMDMD77$.ZMZMM78
+                                                      MMMMMMMMMMMMMMMMMMMZOMMM+Z
+   Static Semantics Theory module:                     MMMMMMMMMMMMMMMMM^NZMMN+Z
+   * boundedness of modular arithmetic outputs,         MMMMMMMMMMMMMMM/.$MZM8O+
+   * type-preservation of operational semantics,         MMMMMMMMMMMMMM7..$MNDM+
+   * progress of memory-safe programs, and                MMDMMMMMMMMMZ7..$DM$77
+   * proof of type-safety.                                 MMMMMMM+MMMZ7..7ZM~++
+                                                            MMMMMMMMMMM7..ZNOOMZ
+   To compile this module, first load and compile:           MMMMMMMMMM$.$MOMO=7
+   * Picinae_core                                             MDMMMMMMMO.7MDM7M+
+   * Picinae_theory                                            ZMMMMMMMM.$MM8$MN
+   Then compile this module with menu option                   $ZMMMMMMZ..MMMOMZ
+   Compile->Compile_buffer.                                     ?MMMMMM7..MNN7$M
+                                                                 ?MMMMMZ..MZM$ZZ
+                                                                  ?$MMMZ7.ZZM7DZ
+                                                                    7MMM$.7MDOD7
+                                                                     7MMM.7M77ZZ
+                                                                      $MM78ZDZ7Z
+                                                                        MM8D$7Z7
+                                                                        MM7O$$+Z
+                                                                         M 7N8ZD
+ *)
+
+Require Import Picinae_theory.
+Require Import NArith.
+Require Import ZArith.
+Require Import Program.Equality.
+Require Import FunctionalExtensionality.
+
+
+
+Section HasUpperBound.
+
+(* Define the has-upper-bound property of pairs of partial functions, and
+   prove some general sufficiency conditions for having the property. *)
+
+Definition has_upper_bound {A B} (f g: A -> option B) :=
+  forall x y z, f x = Some y -> g x = Some z -> y = z.
+
+Lemma hub_refl:
+  forall A B (f: A -> option B), has_upper_bound f f.
+Proof.
+  unfold has_upper_bound. intros.
+  rewrite H0 in H. inversion H.
+  reflexivity.
+Qed.
+
+Lemma hub_sym:
+  forall A B (f g: A -> option B), has_upper_bound f g -> has_upper_bound g f.
+Proof.
+  intros. intros x gx fx H1 H2. symmetry. eapply H; eassumption.
+Qed.
+
+Lemma hub_subset:
+  forall A B (f g f' g': A -> option B) (HUB: has_upper_bound f g)
+         (SS1: f' ⊆ f) (SS2: g' ⊆ g),
+  has_upper_bound f' g'.
+Proof.
+  unfold has_upper_bound. intros. eapply HUB.
+    apply SS1. eassumption.
+    apply SS2. assumption.
+Qed.
+
+Lemma hub_update {A B} {eq:EqDec A}:
+  forall (f g: A -> option B) x y (HUB: has_upper_bound f g),
+  has_upper_bound (f[x:=y]) (g[x:=y]).
+Proof.
+  unfold has_upper_bound. intros. destruct (x0 == x).
+    subst. rewrite update_updated in H,H0. rewrite H0 in H. inversion H. reflexivity.
+    rewrite update_frame in H,H0 by assumption. eapply HUB; eassumption.
+Qed.
+
+End HasUpperBound.
+
+
+
+Module Type PICINAE_STATICS_DEFS (IL: PICINAE_IL) (TIL: PICINAE_THEORY IL).
+
+(* This module proves that the semantics of the IL are type-safe in the sense that
+   programs whose constants have proper bitwidths never produce variable values or
+   expressions that exceed their declared bitwidths as they execute.  This is
+   important for (1) providing assurance that the semantics are correctly defined,
+   and (2) proving practical results that rely upon the assumption that machine
+   registers and memory contents always have values of appropriate bitwidths. *)
+
+Import IL.
+Import TIL.
+Open Scope N.
+
+(* Memory is well-typed if it is 2^w bytes concatenated. *)
+Definition welltyped_memory (m:memory) (w:bitwidth) : Prop :=
+  m < memsize w.
+
+(* Type-check an expression in a typing context, returning its value type. *)
+Inductive hasmtyp_exp (c:mtypctx): exp -> typ -> Prop :=
+| MTVar v t (CV: c v = Some t): hasmtyp_exp c (Var v) t
+| MTWord n w : hasmtyp_exp c (Word n w) NumT
+| MTLoad e1 e2 en len
+        (M1: hasmtyp_exp c e1 MemT) (T2: hasmtyp_exp c e2 NumT):
+        hasmtyp_exp c (Load e1 e2 en len) NumT
+| MTStore e1 e2 e3 en len
+         (M1: hasmtyp_exp c e1 MemT) (T2: hasmtyp_exp c e2 NumT)
+         (M3: hasmtyp_exp c e3 NumT):
+         hasmtyp_exp c (Store e1 e2 e3 en len) MemT
+| MTBinOp bop e1 e2
+         (M1: hasmtyp_exp c e1 NumT) (T2: hasmtyp_exp c e2 NumT):
+         hasmtyp_exp c (BinOp bop e1 e2) NumT
+| MTUnOp uop e (T1: hasmtyp_exp c e NumT):
+        hasmtyp_exp c (UnOp uop e) NumT
+| MTCast ct w' e (T1: hasmtyp_exp c e NumT):
+        hasmtyp_exp c (Cast ct w' e) NumT
+| MTLet v e1 e2 t1 t2
+       (M1: hasmtyp_exp c e1 t1) (T2: hasmtyp_exp (c[v:=Some t1]) e2 t2):
+       hasmtyp_exp c (Let v e1 e2) t2
+| MTUnknown w: hasmtyp_exp c (Unknown w) NumT
+| MTIte e1 e2 e3 t'
+       (M1: hasmtyp_exp c e1 NumT) (T2: hasmtyp_exp c e2 t') (T3: hasmtyp_exp c e3 t'):
+       hasmtyp_exp c (Ite e1 e2 e3) t'
+| MTExtract n1 n2 e1
+           (M1: hasmtyp_exp c e1 NumT):
+           hasmtyp_exp c (Extract n1 n2 e1) NumT
+| MTConcat e1 e2
+          (M1: hasmtyp_exp c e1 NumT) (T2: hasmtyp_exp c e2 NumT):
+          hasmtyp_exp c (Concat e1 e2) NumT.
+
+(* Static semantics for statements:
+   Defining a sound statement typing semantics is tricky for two reasons:
+
+   (1) There are really two kinds of IL variables: (a) those that encode cpu state
+   (which are always initialized, and whose types are fixed), and (b) temporary
+   variables introduced during lifting to IL (which are not guaranteed to be
+   initialized, and whose types may vary across different instruction IL blocks.
+
+   We therefore use separate contexts c0 and c to model the two kinds.  Context
+   c0 models the cpu state variables, while c models all variables.  Context c
+   therefore usually subsumes c0, and is always consistent with c0 (i.e., the
+   join of c and c0 is always a valid context).  This consistency is enforced
+   by checking assigned value types against c0 at every Move, but only updating c.
+
+   (2) Since variable initialization states are mutable, we need static rules
+   that support meets and joins of contexts.  However, a general cut rule is
+   cumbersome because it hampers syntax-directed type-safety proofs.  We therefore
+   instead introduce a weakening option within each syntax-directed typing rule.
+   This avoids superfluous double-cuts by in-lining a single cut into each rule. *)
+
+Inductive hasmtyp_stmt (c0 c:mtypctx): stmt -> mtypctx -> Prop :=
+| MTNop c' (SS: c' ⊆ c): hasmtyp_stmt c0 c Nop c'
+| MTMove v t e c' (CV: c0 v = None \/ c0 v = Some t) (TE: hasmtyp_exp c e t) (SS: c' ⊆ c[v:=Some t]):
+    hasmtyp_stmt c0 c (Move v e) c'
+| MTJmp e c' (TE: hasmtyp_exp c e NumT) (SS: c' ⊆ c): hasmtyp_stmt c0 c (Jmp e) c'
+| MTExn ex c' (SS: c' ⊆ c): hasmtyp_stmt c0 c (Exn ex) c'
+| MTSeq q1 q2 c1 c2 c'
+       (TS1: hasmtyp_stmt c0 c q1 c1) (TS2: hasmtyp_stmt c0 c1 q2 c2) (SS: c' ⊆ c2):
+    hasmtyp_stmt c0 c (Seq q1 q2) c'
+| MTIf e q1 q2 c2 c'
+      (TE: hasmtyp_exp c e NumT)
+      (TS1: hasmtyp_stmt c0 c q1 c2) (TS2: hasmtyp_stmt c0 c q2 c2) (SS: c' ⊆ c2):
+    hasmtyp_stmt c0 c (If e q1 q2) c'
+| MTRep e q c' c''
+    (TE: hasmtyp_exp c e NumT) (SS: c' ⊆ c) (TS: hasmtyp_stmt c0 c' q c') (SS: c'' ⊆ c'):
+    hasmtyp_stmt c0 c (Rep e q) c''.
+
+(* A program is well-typed if all its statements are well-typed. *)
+Definition wellmtyped_prog (c0:mtypctx) (p:program) : Prop :=
+  forall s a, match p s a with None => True | Some (_,q) =>
+                exists c', hasmtyp_stmt c0 c0 q c' end.
+
+(* Context c "models" a store s trivially because numeric and memory
+   types are erased. *)
+Definition mmodels (c:mtypctx) (s:store) : Prop := True.
+
+Theorem models_update:
+  forall c s x y,
+  mmodels c (update s x y).
+Proof.
+  intros; exact I.
+Qed.
+
+(* We next define an effective procedure for type-checking expressions and
+   statements.  This procedure is sound but incomplete: it can determine well-
+   typedness of most statements, but there exist well-typed statements for
+   which it cannot decide their well-typedness.  This happens because the
+   formal semantics above allow arbitrary ("magic") context-weakening within
+   each well-typedness rule, wherein an effective procedure must guess
+   the greatest-lower-bound context sufficient to type-check the remainder of
+   the statement.  The procedure below makes the following guesses, which
+   suffice to prove well-typedness for IL encodings of all ISAs so far:
+     (1) If-contexts are weakened to the lattice-meet of the two branches.
+     (2) Rep-contexts are weakened to the input context, to get a fixpoint.
+     (3) No other contexts are weakened.
+   If these guesses cannot typecheck some statements in your ISA, consider
+   changing your lifter for your ISA to produce IL encodings whose variable
+   types are not path-sensitive. *)
+
+(* Type-check an expression in a given typing context. *)
+Fixpoint mtypchk_exp (e:exp) (c:mtypctx): option typ :=
+  match e with
+  | Var v => c v
+  | Word n w => Some NumT
+  | Load e1 e2 _ len =>
+      match mtypchk_exp e1 c, mtypchk_exp e2 c with
+      | Some MemT, Some NumT => Some NumT
+      | _, _ => None
+      end
+  | Store e1 e2 e3 _ len =>
+      match mtypchk_exp e1 c, mtypchk_exp e2 c, mtypchk_exp e3 c with
+      | Some MemT, Some NumT, Some NumT => Some MemT
+      | _, _, _ => None
+      end
+  | BinOp bop e1 e2 =>
+      match mtypchk_exp e1 c, mtypchk_exp e2 c with
+      | Some NumT, Some NumT => Some NumT
+      | _, _ => None
+      end
+  | UnOp uop e1 => match mtypchk_exp e1 c with Some NumT => Some NumT
+                                            | _ => None end
+  | Cast ct w' e1 =>
+      match mtypchk_exp e1 c with Some NumT => Some NumT
+      | _ => None
+      end
+  | Let v e1 e2 =>
+      match mtypchk_exp e1 c with Some w => mtypchk_exp e2 (c[v:=Some w])
+                               | None => None end
+  | Unknown w => Some NumT
+  | Ite e1 e2 e3 =>
+      match mtypchk_exp e1 c, mtypchk_exp e2 c, mtypchk_exp e3 c with
+      | Some NumT, Some w2, Some w3 => if w2 == w3 then Some w2 else None
+      | _, _, _ => None
+      end
+  | Extract n1 n2 e1 =>
+      match mtypchk_exp e1 c with
+      | Some NumT => Some NumT
+      | _ => None
+      end
+  | Concat e1 e2 =>
+      match mtypchk_exp e1 c, mtypchk_exp e2 c with
+      | Some NumT, Some NumT => Some NumT
+      | _, _ => None
+      end
+  end.
+
+
+(* Compute the meet of two input contexts. *)
+Definition mtypctx_meet {B:Type} {E:EqDec B} (c1 c2:var -> option B) v :=
+  match c1 v, c2 v with
+  | Some w1, Some w2 => if w1 == w2 then Some w1 else None
+  | _, _ => None
+  end.
+
+(* Type-check a statement given a frame-context and initial context. *)
+Fixpoint mtypchk_stmt (q:stmt) (c0 c:mtypctx): option mtypctx :=
+  match q with
+  | Nop => Some c
+  | Move v e =>
+      match mtypchk_exp e c with
+      | Some t => match c0 v with
+                  | None => Some (c[v:=Some t])
+                  | Some t' => if t == t' then Some (c[v:=Some t]) else None
+                  end
+      | None => None
+      end
+  | Jmp e => match mtypchk_exp e c with Some NumT => Some c | _ => None end
+  | Exn _ => Some c
+  | Seq q1 q2 => match mtypchk_stmt q1 c0 c with
+                 | None => None
+                 | Some c2 => mtypchk_stmt q2 c0 c2
+                 end
+  | If e q1 q2 =>
+      match mtypchk_exp e c, mtypchk_stmt q1 c0 c, mtypchk_stmt q2 c0 c with
+      | Some NumT, Some c1, Some c2 => Some (mtypctx_meet c1 c2)
+      | _, _, _ => None
+      end
+  | Rep e q1 =>
+      match mtypchk_exp e c, mtypchk_stmt q1 c c with
+      | Some NumT, Some _ => Some c
+      | _, _ => None
+      end
+  end.
+
+End PICINAE_STATICS_DEFS.
+
+
+
+Module Type PICINAE_STATICS (IL: PICINAE_IL) (TIL: PICINAE_THEORY IL).
+
+Import IL.
+Import TIL.
+Include PICINAE_STATICS_DEFS IL TIL.
+
+(* These short lemmas are helpful when automating type-checking in tactics. *)
+
+(* Expression types are unique. *)
+Parameter hasmtyp_exp_unique:
+  forall e c1 c2 t1 t2 (HUB: has_upper_bound c1 c2)
+         (TE1: hasmtyp_exp c1 e t1) (TE2: hasmtyp_exp c2 e t2),
+  t1 = t2.
+
+(* Expression typing contexts can be weakened. *)
+Parameter hasmtyp_exp_weaken:
+  forall c1 c2 e t (TE: hasmtyp_exp c1 e t) (SS: c1 ⊆ c2),
+  hasmtyp_exp c2 e t.
+
+(* Statement types can be weakened. *)
+Parameter hasmtyp_stmt_weaken:
+  forall c0 c1 c2 c' q (TS: hasmtyp_stmt c0 c1 q c') (SS: c1 ⊆ c2),
+  hasmtyp_stmt c0 c2 q c'.
+Parameter hasmtyp_stmt_weaken':
+  forall c0 c c' c'' q (TS: hasmtyp_stmt c0 c q c') (SS: c'' ⊆ c'),
+  hasmtyp_stmt c0 c q c''.
+
+(* Statement types agree (though not necessarily unique). *)
+Parameter hasmtyp_stmt_compat:
+  forall c0 q c1 c2 c1' c2'
+         (HUB: has_upper_bound c1 c2)
+         (TS1: hasmtyp_stmt c0 c1 q c1') (TS2: hasmtyp_stmt c0 c2 q c2'),
+  has_upper_bound c1' c2'.
+
+(* Statement frame contexts can be weakened. *)
+Parameter hasmtyp_stmt_frame_weaken:
+  forall c0 c0' q c c' (TS: hasmtyp_stmt c0 c q c') (SS: c0' ⊆ c0),
+  hasmtyp_stmt c0' c q c'.
+
+(* We next prove type-safety of the IL with respect to the above static semantics.
+   In general, interpretation of an arbitrary, unchecked IL program can fail
+   (i.e., exec_prog is underivable) for only the following reasons:
+
+   (1) memory access violation ("mem_readable" or "mem_writable" is falsified), or
+
+   (2) a type-mismatch occurs (e.g., arithmetic applied to memory state values).
+
+   Type-safety proves that if type-checking succeeds, then the only reachable
+   stuck-states are case (1).  That is, runtime type-mismatches are precluded,
+   and all computed values have proper types.
+
+   This property is important in the context of formal validation of native
+   code programs because proofs about such code typically rely upon the types
+   of values that each cpu state element can hold (e.g., 32-bit registers always
+   contain 32-bit numbers).  Proving type-safety allows us to verify these
+   basic properties within other proofs by first running the type-checker (as a
+   tactic), and then applying the type-soundness theorem(s). *)
+
+
+(* Weakening the typing context preserves the modeling relation. *)
+Parameter models_subset:
+  forall c s c' (M: mmodels c s) (SS: c' ⊆ c),
+  mmodels c' s.
+
+(* The expression type-checker is sound. *)
+Parameter mtypchk_exp_sound:
+  forall e c t, mtypchk_exp e c = Some t -> hasmtyp_exp c e t.
+
+(* The meet of two contexts is bounded above by the contexts. *)
+Parameter mtypctx_meet_subset:
+  forall {B:Type} {E:EqDec B} c1 c2, mtypctx_meet c1 c2 ⊆ c1.
+
+(* Context-meet is commutative. *)
+Parameter mtypctx_meet_comm:
+  forall {B} {E:EqDec B} c1 c2, mtypctx_meet c1 c2 = mtypctx_meet c2 c1.
+
+(* Context-meet computes the greatest of the lower bounds of the inputs. *)
+Parameter mtypctx_meet_lowbound:
+  forall {B} {E:EqDec B} c0 c1 c2 (SS1: c0 ⊆ c1) (SS2: c0 ⊆ c2), c0 ⊆ mtypctx_meet c1 c2.
+
+(* The type-checker preserves the frame context. *)
+Parameter mtypchk_stmt_mono:
+  forall c0 q c c' (TS: mtypchk_stmt q c0 c = Some c') (SS: c0 ⊆ c), c0 ⊆ c'.
+
+(* The statement type-checker is sound. *)
+Parameter mtypchk_stmt_sound:
+  forall q c0 c c' (SS: c0 ⊆ c) (TS: mtypchk_stmt q c0 c = Some c'),
+  hasmtyp_stmt c0 c q c'.
+
+(* Create a theorem that transforms a type-safety goal into an application of
+   the type-checker.  This allows type-safety goals to be solved by any of
+   Coq's fast reduction tactics, such as vm_compute or native_compute. *)
+Parameter mtypchk_stmt_compute:
+  forall q c (TS: if mtypchk_stmt q c c then True else False),
+  exists c', hasmtyp_stmt c c q c'.
+
+(* Attempt to automatically solve a goal of the form (welltyped_prog c p).
+   Statements in p that cannot be type-checked automatically (using context-
+   meets at conditionals and the incoming context as the fixpoint of loops)
+   are left as subgoals for the user to solve.  For most ISAs, this should
+   not happen; the algorithm should fully solve all the goals. *)
+Ltac Picinae_mtypecheck :=
+  lazymatch goal with [ |- wellmtyped_prog _ _ ] =>
+    let s := fresh "s" in let a := fresh "a" in
+    intros s a;
+    destruct a as [|a]; repeat first [ exact I | destruct a as [a|a|] ];
+    try (apply mtypchk_stmt_compute; vm_compute; exact I)
+  | _ => fail "goal is not of the form (welltyped_prog c p)"
+  end.
+
+End PICINAE_STATICS.
+
+
+Module PicinaeMStatics (IL: PICINAE_IL) (TIL: PICINAE_THEORY IL): PICINAE_STATICS IL TIL.
+
+Import IL.
+Import TIL.
+Include PICINAE_STATICS_DEFS IL TIL.
+
+Lemma hasmtyp_binop:
+  forall bop c e1 e2
+         (T1: hasmtyp_exp c e1 NumT) (T2: hasmtyp_exp c e2 NumT),
+  hasmtyp_exp c (BinOp bop e1 e2) NumT.
+Proof.
+  intros. econstructor; assumption.
+Qed.
+
+Lemma hasmtyp_extract:
+  forall c n1 n2 e1
+         (T1: hasmtyp_exp c e1 NumT),
+  hasmtyp_exp c (Extract n1 n2 e1) NumT.
+Proof.
+  intros. econstructor; assumption.
+Qed.
+
+Lemma hasmtyp_concat:
+  forall c e1 e2
+         (T1: hasmtyp_exp c e1 NumT) (T2: hasmtyp_exp c e2 NumT),
+  hasmtyp_exp c (Concat e1 e2) NumT.
+Proof.
+  intros. econstructor; assumption.
+Qed.
+
+Theorem hasmtyp_exp_unique:
+  forall e c1 c2 w1 w2 (HUB: has_upper_bound c1 c2)
+         (TE1: hasmtyp_exp c1 e w1) (TE2: hasmtyp_exp c2 e w2),
+  w1 = w2.
+Proof.
+  intros. revert c1 c2 w1 w2 HUB TE1 TE2. induction e; intros;
+  inversion TE1; inversion TE2; clear TE1 TE2; subst;
+  try reflexivity.
+
+  (* Var *)
+  eapply HUB; eassumption.
+
+  (* ? *)
+  specialize (IHe1 _ _ _ _ HUB M1 M0); subst t0. apply (hub_update _ _ v (Some t1)) in HUB.
+  specialize (IHe2 _ _ _ _ HUB T2 T0); now subst.
+
+  (* ? *)
+  specialize (IHe2 _ _ _ _ HUB T2 T0); now subst.
+Qed.
+
+Theorem hasmtyp_exp_weaken:
+  forall c1 c2 e t (TE: hasmtyp_exp c1 e t) (SS: c1 ⊆ c2),
+  hasmtyp_exp c2 e t.
+Proof.
+  intros. revert c2 SS. dependent induction TE; intros; econstructor;
+  try (try first [ apply IHTE | apply IHTE1 | apply IHTE2 | apply IHTE3 | apply SS ]; assumption).
+
+  apply IHTE2. unfold update. intros v0 t CV. destruct (v0 == v).
+    assumption.
+    apply SS. assumption.
+Qed.
+
+Theorem hasmtyp_stmt_weaken':
+  forall c0 c c' c'' q (TS: hasmtyp_stmt c0 c q c') (SS: c'' ⊆ c'),
+  hasmtyp_stmt c0 c q c''.
+Proof.
+  intros. inversion TS; clear TS; subst;
+  econstructor; first [ eassumption | transitivity c'; assumption ].
+Qed.
+
+Theorem hasmtyp_stmt_weaken:
+  forall c0 c1 c2 c' q (TS: hasmtyp_stmt c0 c1 q c') (SS: c1 ⊆ c2),
+  hasmtyp_stmt c0 c2 q c'.
+Proof.
+  intros. revert c2 SS. dependent induction TS; intros;
+  try solve [ econstructor; repeat first
+  [ eassumption
+  | eapply hasmtyp_exp_weaken; eassumption
+  | apply pfsub_update; assumption
+  | (apply IHTS1 + apply IHTS2); assumption
+  | etransitivity; [eassumption|] ] ].
+
+  econstructor.
+    eapply hasmtyp_exp_weaken; eassumption.
+    etransitivity; [|eassumption]. eassumption.
+    apply IHTS. reflexivity.
+    assumption.
+Qed.
+
+Theorem hasmtyp_stmt_compat:
+  forall c0 q c1 c2 c1' c2'
+         (HUB: has_upper_bound c1 c2)
+         (TS1: hasmtyp_stmt c0 c1 q c1') (TS2: hasmtyp_stmt c0 c2 q c2'),
+  has_upper_bound c1' c2'.
+Proof.
+  induction q; intros; inversion TS1; inversion TS2; clear TS1 TS2; subst;
+  try solve [ apply (hub_subset _ _ _ _ _ _ HUB); assumption ].
+    eapply hub_subset; [|eassumption..]. replace t0 with t.
+      apply hub_update, HUB.
+      eapply hasmtyp_exp_unique; eassumption.
+    eapply IHq2.
+      eapply IHq1; eassumption.
+      eapply hasmtyp_stmt_weaken'. exact TS3. exact SS.
+      eapply hasmtyp_stmt_weaken'. exact TS5. exact SS0.
+    eapply hub_subset; [|eassumption..]. eapply IHq1; eassumption.
+    eapply IHq; [eassumption| |];
+      (eapply hasmtyp_stmt_weaken; [|eassumption]);
+      eapply hasmtyp_stmt_weaken'; eassumption.
+Qed.
+
+Theorem hasmtyp_stmt_frame_weaken:
+  forall c0 c0' q c c' (TS: hasmtyp_stmt c0 c q c') (SS: c0' ⊆ c0),
+  hasmtyp_stmt c0' c q c'.
+Proof.
+  induction q; intros; inversion TS; subst.
+    apply MTNop. assumption.
+    eapply MTMove.
+      specialize (SS v). destruct (c0' v).
+        right. rewrite (SS t0 (eq_refl _)) in CV. destruct CV. discriminate. eassumption.
+        left. reflexivity.
+      exact TE.
+      assumption.
+    eapply MTJmp. exact TE. assumption.
+    apply MTExn. assumption.
+    eapply MTSeq.
+      apply IHq1. exact TS1. exact SS.
+      apply IHq2. exact TS2. exact SS.
+      exact SS0.
+    eapply MTIf.
+      exact TE.
+      apply IHq1. exact TS1. exact SS.
+      apply IHq2. exact TS2. exact SS.
+      exact SS0.
+    eapply MTRep.
+      exact TE.
+      exact SS0.
+      apply IHq. exact TS0. exact SS.
+      exact SS1.
+Qed.
+
+Lemma models_subset:
+  forall c s c' (M: mmodels c s) (SS: c' ⊆ c),
+  mmodels c' s.
+Proof.
+  intros; exact I.
+Qed.
+
+Lemma models_reset_temps:
+  forall s2 s1 (MDL: mmodels marchtyps s2), mmodels marchtyps (reset_temps s1 s2).
+Proof.
+  intros; exact I.
+Qed.
+
+Remark shiftl1_3pn:
+  forall n, N.shiftl 1 (3+n) = 2^n*8.
+Proof.
+  intro. rewrite N.shiftl_1_l, N.pow_add_r, N.mul_comm. reflexivity.
+Qed.
+
+Theorem mtypchk_exp_sound:
+  forall e c t, mtypchk_exp e c = Some t -> hasmtyp_exp c e t.
+Proof.
+  induction e; cbn [ mtypchk_exp ]; intros.
+
+  (* Var *)
+  apply MTVar. assumption.
+
+  (* Word *)
+  injection H; intro; subst. apply MTWord.
+
+  (* Load *)
+  specialize (IHe1 c). specialize (IHe2 c).
+  destruct (mtypchk_exp e1 c) as [[ | ]|]; try discriminate.
+  destruct (mtypchk_exp e2 c) as [[ | ]|]; try discriminate.
+  inversion H; subst.
+  eapply MTLoad.
+    apply IHe1. reflexivity.
+    apply IHe2. reflexivity.
+
+  (* Store *)
+  specialize (IHe1 c). specialize (IHe2 c). specialize (IHe3 c).
+  destruct (mtypchk_exp e1 c) as [[|]|]; try discriminate.
+  destruct (mtypchk_exp e2 c) as [[|]|]; try discriminate.
+  destruct (mtypchk_exp e3 c) as [[|]|]; try discriminate.
+  inversion H; subst; clear H.
+  apply MTStore.
+    apply IHe1. reflexivity.
+    apply IHe2. reflexivity.
+    apply IHe3. reflexivity.
+
+  (* BinOp *)
+  specialize (IHe1 c). specialize (IHe2 c).
+  destruct (mtypchk_exp e1 c) as [[|]|]; try discriminate.
+  destruct (mtypchk_exp e2 c) as [[|]|]; try discriminate.
+  inversion H; subst; clear H.
+  apply MTBinOp.
+    apply IHe1. reflexivity.
+    apply IHe2. reflexivity.
+
+  (* UnOp *)
+  specialize (IHe c).
+  destruct (mtypchk_exp e c) as [[|]|]; try discriminate.
+  injection H; intro; subst.
+  apply MTUnOp. apply IHe. reflexivity.
+
+  (* Cast *)
+  specialize (IHe c0).
+  destruct (mtypchk_exp e c0) as [[|]|]; try discriminate.
+  inversion H; subst; clear H.
+  (eapply MTCast; eapply IHe; reflexivity).
+
+  (* Let *)
+  specialize (IHe1 c). destruct (mtypchk_exp e1 c); [|discriminate].
+  eapply MTLet.
+    apply IHe1. reflexivity.
+    apply IHe2. assumption.
+
+  (* Unknown *)
+  injection H; intro; subst. apply MTUnknown.
+
+  (* Ite *)
+  specialize (IHe1 c). specialize (IHe2 c). specialize (IHe3 c).
+  destruct (mtypchk_exp e1 c) as [[|]|]; try discriminate.
+  destruct (mtypchk_exp e2 c) as [[|]|]; try discriminate;
+  destruct (mtypchk_exp e3 c) as [[|]|]; try discriminate;
+  injection H; intro; subst.
+  eapply MTIte.
+    apply IHe1. reflexivity.
+    apply IHe2. reflexivity.
+    apply IHe3. reflexivity.
+  eapply MTIte.
+    apply IHe1. reflexivity.
+    apply IHe2. reflexivity.
+    apply IHe3. reflexivity.
+
+  (* Extract *)
+  specialize (IHe c).
+  destruct (mtypchk_exp e c) as [[|]|]; try discriminate.
+  injection H; intro; subst.
+  eapply MTExtract.
+    apply IHe. reflexivity.
+
+  (* Concat *)
+  specialize (IHe1 c). specialize (IHe2 c).
+  destruct (mtypchk_exp e1 c) as [[|]|]; try discriminate.
+  destruct (mtypchk_exp e2 c) as [[|]|]; try discriminate.
+  injection H; intro; subst.
+  apply MTConcat.
+    apply IHe1. reflexivity.
+    apply IHe2. reflexivity.
+Qed.
+
+Lemma mtypctx_meet_subset {B} {E:EqDec B}:
+  forall c1 c2, mtypctx_meet c1 c2 ⊆ c1.
+Proof.
+  intros c1 c2 v t H. unfold mtypctx_meet in H.
+  destruct (c1 v) as [t1|]; [|discriminate].
+  destruct (c2 v) as [t2|]; [|discriminate].
+  destruct (t1 == t2). exact H. discriminate.
+Qed.
+
+Lemma mtypctx_meet_comm {B} {E:EqDec B}:
+  forall c1 c2, mtypctx_meet c1 c2 = mtypctx_meet c2 c1.
+Proof.
+  intros. extensionality v. unfold mtypctx_meet.
+  destruct (c1 v) as [w1|], (c2 v) as [w2|]; try reflexivity.
+  destruct (w1 == w2).
+    subst. destruct (w2 == w2). reflexivity. contradict n. reflexivity.
+    destruct (w2 == w1). contradict n. symmetry. assumption. reflexivity.
+Qed.
+
+Lemma mtypctx_meet_lowbound {B} {E:EqDec B}:
+  forall (c0 c1 c2:var->option B) (SS1: c0 ⊆ c1) (SS2: c0 ⊆ c2), c0 ⊆ mtypctx_meet c1 c2.
+Proof.
+  unfold "⊆", mtypctx_meet. intros.
+  rewrite (SS1 _ _ H). rewrite (SS2 _ _ H).
+  destruct (y == y); [|contradict n]; reflexivity.
+Qed.
+
+Lemma mtypchk_stmt_mono:
+  forall c0 q c c' (TS: mtypchk_stmt q c0 c = Some c') (SS: c0 ⊆ c), c0 ⊆ c'.
+Proof.
+  induction q; simpl; intros.
+
+  (* Nop *)
+  injection TS; intro; subst. exact SS.
+
+  (* Move *)
+  destruct (mtypchk_exp e c) as [w|]; [|discriminate].
+  destruct (c0 v) as [w'|] eqn:C0V.
+    destruct (w == w').
+      injection TS; intro; subst. intros v0 t0 H. destruct (v0 == v).
+        subst v0. rewrite update_updated, <- C0V, <- H. reflexivity.
+        rewrite update_frame by assumption. apply SS, H.
+      discriminate.
+    injection TS; intro; subst. intros v0 t0 H. destruct (v0 == v).
+      subst v0. rewrite C0V in H. discriminate.
+      rewrite update_frame by assumption. apply SS, H.
+
+  (* Jmp *)
+  destruct (mtypchk_exp e c) as [[|]|]; try discriminate.
+  injection TS; intro; subst. exact SS.
+
+  (* Exn *)
+  injection TS; intro; subst. exact SS.
+
+  (* Seq *)
+  destruct (mtypchk_stmt q1 c0 c) as [c1|] eqn:TS1; [|discriminate].
+  eapply IHq2. exact TS.
+  eapply IHq1. exact TS1. exact SS.
+
+  (* If *)
+  destruct (mtypchk_exp e c) as [[|]|]; try discriminate.
+  destruct (mtypchk_stmt q1 c0 c) as [c1|] eqn:TS1; [|discriminate].
+  destruct (mtypchk_stmt q2 c0 c) as [c2|] eqn:TS2; [|discriminate].
+  injection TS; intro; subst.
+  apply mtypctx_meet_lowbound.
+    eapply IHq1. exact TS1. exact SS.
+    eapply IHq2. exact TS2. exact SS.
+
+  (* Rep *)
+  destruct (mtypchk_exp e c) as [[|]|]; try discriminate.
+  destruct (mtypchk_stmt q c c) eqn:TS1; try discriminate.
+  injection TS; intro; subst.
+  exact SS.
+Qed.
+
+Theorem mtypchk_stmt_sound:
+  forall q c0 c c' (SS: c0 ⊆ c) (TS: mtypchk_stmt q c0 c = Some c'),
+  hasmtyp_stmt c0 c q c'.
+Proof.
+  induction q; intros; simpl in TS.
+
+  (* Nop *)
+  injection TS; intro; subst. apply MTNop. reflexivity.
+
+  (* Move *)
+  destruct (mtypchk_exp e c) as [|] eqn:TE; try discriminate.
+  destruct (c0 v) as [t'|] eqn:C0V.
+    destruct (t==t'); try discriminate. inversion TS; subst.
+    econstructor. right; eassumption. apply mtypchk_exp_sound; assumption. reflexivity.
+
+    inversion TS; subst. econstructor. left; assumption. apply mtypchk_exp_sound. eassumption. reflexivity.
+
+  (* Jmp *)
+  destruct (mtypchk_exp e c) as [[|]|] eqn:TE; try discriminate.
+  injection TS; intro; subst.
+  eapply MTJmp. apply mtypchk_exp_sound. exact TE. reflexivity.
+
+  (* Exn *)
+  injection TS; intro; subst. apply MTExn. reflexivity.
+
+  (* Seq *)
+  specialize (IHq1 c0 c). destruct (mtypchk_stmt q1 c0 c) as [c1|] eqn:TS1; [|discriminate].
+  specialize (IHq2 c0 c1). destruct (mtypchk_stmt q2 c0 c1); [|discriminate].
+  injection TS; clear TS; intro; subst.
+  eapply MTSeq.
+    apply IHq1. exact SS. reflexivity.
+    apply IHq2. eapply mtypchk_stmt_mono; eassumption. reflexivity. reflexivity.
+
+  (* If *)
+  destruct (mtypchk_exp e c) as [[|]|] eqn:TE; try discriminate.
+  destruct (mtypchk_stmt q1 c0 c) as [c1|] eqn:TS1; [|discriminate].
+  destruct (mtypchk_stmt q2 c0 c) as [c2|] eqn:TS2; [|discriminate].
+  injection TS; clear TS; intro; subst.
+  eapply MTIf.
+    apply mtypchk_exp_sound. exact TE.
+    eapply hasmtyp_stmt_weaken'.
+      apply IHq1. exact SS. exact TS1.
+      apply mtypctx_meet_subset.
+    eapply hasmtyp_stmt_weaken'.
+      apply IHq2. exact SS. exact TS2.
+      rewrite mtypctx_meet_comm. apply mtypctx_meet_subset.
+    reflexivity.
+
+  (* Rep *)
+  destruct (mtypchk_exp e c) as [[|]|] eqn:TE; try discriminate.
+  specialize (IHq c c). destruct (mtypchk_stmt q c c) as [c1|] eqn:TS1; [|discriminate].
+  injection TS; clear TS; intro; subst.
+  eapply MTRep.
+    apply mtypchk_exp_sound. exact TE.
+    reflexivity.
+    eapply hasmtyp_stmt_frame_weaken; [|exact SS]. eapply hasmtyp_stmt_weaken'.
+      apply IHq. reflexivity. reflexivity.
+      eapply mtypchk_stmt_mono. exact TS1. reflexivity.
+    reflexivity.
+Qed.
+
+Corollary mtypchk_stmt_compute:
+  forall q c (TS: if mtypchk_stmt q c c then True else False),
+  exists c', hasmtyp_stmt c c q c'.
+Proof.
+  intros. destruct (mtypchk_stmt q c c) as [c'|] eqn:TS1.
+    exists c'. apply mtypchk_stmt_sound. reflexivity. exact TS1.
+    contradict TS.
+Qed.
+
+End PicinaeMStatics.
